Finish proof of sortedness

src/two_tree.lean
@@ -1,33 +1,13 @@
-import tactic.default .tactic
+import tactic.default .tactic .basic
 universes u v w
 
 namespace two_three
 
 variables (α : Type u) (β : Type v) {γ : Type w}
 
-inductive tree
-| leaf (k : α) (v : β)
-| node2 (t₀ : tree) (x : α) (t₁ : tree)
-| node3 (t₀ : tree) (x : α) (t₁ : tree) (y : α) (t₂ : tree)
--- | node4 (t₀ : tree) (x : α)
---         (t₁ : tree) (y : α)
---         (t₂ : tree) (z : α)
---         (t₃ : tree)
-
 open tree nat
 
 variables {α β}
-
-def first : tree α β → α
-| (tree.leaf x _) := x
-| (tree.node2 t₀ x _) := first t₀
-| (tree.node3 t₀ x _ _ _) := first t₀
-
-def last : tree α β → α
-| (tree.leaf x _) := x
-| (tree.node2 _ x t₁) := last t₁
-| (tree.node3 t₀ x _ _ t₂) := last t₂
--- | (tree.node4 t₀ x _ _ _ _ _) := first t₀
 
 inductive liftp (p : α → Prop) : tree α β → Prop
 | leaf {k v} : p k → liftp (tree.leaf k v)
@@ -67,45 +47,6 @@ section defs
 variables [has_le α] [has_lt α]
 
 open tree nat
-
-inductive below : option α → α → Prop
-| nil {x} : below none x
-| le {x} : below (some x) x
--- | le {x y} : x ≤ y → below (some x) y
-
-inductive above : α → option α → Prop
-| nil {x} : above x none
-| le {x y} : x < y → above x (some y)
-
-inductive sorted' : tree α β → Prop
-| leaf {k v} : sorted' (tree.leaf k v)
-| node2 {x t₀ t₁} :
-  last t₀ < x →
-  x = first t₁ →
-  sorted' t₀ →
-  sorted' t₁ →
-  sorted' (tree.node2 t₀ x t₁)
-| node3 {x y t₀ t₁ t₂} :
-  last t₀ < x →
-  x = first t₁ →
-  last t₁ < y →
-  y = first t₂ →
-  sorted' t₀ →
-  sorted' t₁ →
-  sorted' t₂ →
-  sorted' (tree.node3 t₀ x t₁ y t₂)
-
-inductive with_height : ℕ → tree α β → Prop
-| leaf {k v} : with_height 0 (tree.leaf k v)
-| node2 {n x t₀ t₁} :
-  with_height n t₀ →
-  with_height n t₁ →
-  with_height (succ n) (tree.node2 t₀ x t₁)
-| node3 {n x y t₀ t₁ t₂} :
-  with_height n t₀ →
-  with_height n t₁ →
-  with_height n t₂ →
-  with_height (succ n) (tree.node3 t₀ x t₁ y t₂)
 
 variables [@decidable_rel α (<)]
 
@@ -225,21 +166,33 @@ begin
   repeat { solve_by_elim [le_of_lt] <|> transitivity },
 end
 
+lemma eq_of_below {x : option α} {y : α} (h : below x y) : x.get_or_else y = y :=
+by cases h; refl
+
 lemma above_of_above_of_le {x y : α} {k}
   (h : x ≤ y) (h' : above y k) : above x k :=
 by cases h'; constructor; solve_by_elim [lt_of_le_of_lt]
 
 @[interactive]
 meta def interactive.saturate : tactic unit := do
-tactic.interactive.casesm (some ()) [``(above _ (some _)), ``(below (some _) _)],
+tactic.interactive.casesm (some ()) [``(above _ (some _)), ``(below (some _) _), ``(below' (some _) _)],
 tactic.find_all_hyps ``(sorted' _) $ λ h, do
-  n ← tactic.get_unused_name `h,
+{ n ← tactic.get_unused_name `h,
   tactic.mk_app ``first_le_last_of_sorted [h] >>= tactic.note n none,
-  tactic.skip
+  tactic.skip },
+tactic.find_all_hyps ``(below _ _) $ λ h, do
+{ n ← tactic.get_unused_name `h,
+  tactic.mk_app ``eq_of_below [h] >>= tactic.note n none,
+  tactic.skip },
+tactic.find_all_hyps ``(¬ _ < _) $ λ h, do
+{ -- n ← tactic.get_unused_name `h,
+  tactic.mk_app ``le_of_not_gt [h] >>= tactic.note h.local_pp_name none,
+  tactic.clear h,
+  tactic.skip }
 
 @[interactive]
 meta def interactive.above : tactic unit := do
-tactic.interactive.saturate,
+-- tactic.interactive.saturate,
 tactic.find_hyp ``(above _ _) $ λ h, do
   tactic.refine ``(above_of_above_of_le _ %%h),
   tactic.interactive.chain_trans
