src/zipper.lean
@@ -1,37 +1,9 @@
 
-import .two_tree
+import .basic .backtrack
 
--- namespace tactic
--- open environment
-
--- meta def foo (n : name) (e t : expr) (vs : list expr) : tactic (list intro_rule) := _
-
--- @[user_attribute]
--- meta def mk_zipper_attr : user_attribute :=
--- { name := `zipper,
---   descr := "Make zippers for inductive types",
---   after_set := some $ λ n _ _, do
---     env ← get_env,
---     d ← get_decl n,
---     let ls := d.univ_levels,
---     let e : expr := expr.const n ls,
---     (vs, t) ← infer_type e >>= mk_local_pis,
---     let xs := env.constructors_of n,
---     let n' := n <.> "zipper",
---     xs.mmap $ λ h, do {
---       trace h,
---       let c : expr := expr.const h ls,
---       infer_type (c.mk_app vs) >>= trace },
---     opt ← get_options,
---     updateex_env $ λ e, e.add_ginductive opt d.univ_params vs [((n', t), _)] ff
-
---  }
-
--- end tactic
 universes u v
 variables (α : Type u) (β : Type v)
--- attribute [zipper] tree
-#check two_three.tree
+
 namespace two_three.tree
 open two_three
 
@@ -47,21 +19,23 @@ variables {α β}
 
 namespace zipper
 
-def close : zipper α β → tree α β → tree α β
-| nil t := t
-| (node2_0 z  x t₁) t := close z $ node2 t  x t₁
-| (node2_1 t₀ x z)  t := close z $ node2 t₀ x t
-| (node3_0 z  x t₁ y t₂) t := close z $ node3 t  x t₁ y t₂
-| (node3_1 t₀ x z  y t₂) t := close z $ node3 t₀ x t  y t₂
-| (node3_2 t₀ x t₁ y z)  t := close z $ node3 t₀ x t₁ y t
-.
-def split : zipper α β → tree α β → α → tree α β → tree α β
-| nil ta a tb := node2 ta a tb
-| (node2_0 z  x t₁) ta a tb := close z $ node3 ta a tb x t₁
-| (node2_1 t₀ x z)  ta a tb := close z $ node3 t₀ x ta a tb
-| (node3_0 z  x t₁ y t₂) ta a tb := split z (node2 ta a tb) x (node2 t₁ y t₂)
-| (node3_1 t₀ x z  y t₂) ta a tb := split z (node2 t₀ x ta) a (node2 tb y t₂)
-| (node3_2 t₀ x t₁ y z)  ta a tb := split z (node2 t₀ x t₁) y (node2 ta a tb)
+@[pp_nodot]
+def close : zipper α β → option α → tree α β → tree α β
+| nil k t := t
+| (node2_0 z  x t₁) k t := close z k $ node2 t  x t₁
+| (node2_1 t₀ x z)  k t := close z none $ node2 t₀ (k.get_or_else x) t
+| (node3_0 z  x t₁ y t₂) k t := close z k $ node3 t  x t₁ y t₂
+| (node3_1 t₀ x z  y t₂) k t := close z none $ node3 t₀ (k.get_or_else x) t  y t₂
+| (node3_2 t₀ x t₁ y z)  k t := close z none $ node3 t₀ x t₁ (k.get_or_else y) t
+
+@[pp_nodot]
+def split : zipper α β → option α → tree α β → α → tree α β → tree α β
+| nil k ta a tb := node2 ta a tb
+| (node2_0 z  x t₁) k ta a tb := close z k $ node3 ta a tb x t₁
+| (node2_1 t₀ x z)  k ta a tb := close z none $ node3 t₀ (k.get_or_else x) ta a tb
+| (node3_0 z  x t₁ y t₂) k ta a tb := split z k (node2 ta a tb) x (node2 t₁ y t₂)
+| (node3_1 t₀ x z  y t₂) k ta a tb := split z none (node2 t₀ (k.get_or_else x) ta) a (node2 tb y t₂)
+| (node3_2 t₀ x t₁ y z)  k ta a tb := split z none (node2 t₀ x t₁) (k.get_or_else y) (node2 ta a tb)
 
 section eqv
 
@@ -70,9 +44,9 @@ variables [has_lt α] [@decidable_rel α has_lt.lt]
 def insert (k : α) (v : β) : zipper α β → tree α β → tree α β
 | xs (leaf k' v') :=
   match cmp k k' with
-  | ordering.lt := split xs (tree.leaf k v) k' (tree.leaf k' v')
-  | ordering.eq := close xs (tree.leaf k' v)
-  | ordering.gt := split xs (tree.leaf k' v') k (tree.leaf k v)
+  | ordering.lt := split xs (some k) (tree.leaf k v) k' (tree.leaf k' v')
+  | ordering.eq := close xs (some k') (tree.leaf k' v)
+  | ordering.gt := split xs (some k') (tree.leaf k' v') k (tree.leaf k v)
   end
 | xs (node2 t₀ x t₁) :=
   if k < x
@@ -85,23 +59,13 @@ def insert (k : α) (v : β) : zipper α β → tree α β → tree α β
     then insert (node3_1 t₀ x xs y t₂) t₁
     else insert (node3_2 t₀ x t₁ y xs) t₂
 
-variables [has_le α]
-variables {k : α} {v : β} {t : tree α β} {z : zipper α β}
-
-local attribute [simp] insert insert'
-
-example : insert k v z t = insert' k v t (close z) (split z) :=
-begin
-  induction t generalizing z; dsimp,
-  { cases cmp k t_k; dsimp; refl, },
-  { split_ifs; simp *; refl },
-  { split_ifs; simp *; refl },
-end
+def insert' (k : α) (v : β) : tree α β → tree α β :=
+insert k v zipper.nil
 
 end eqv
 open nat
 
-variables {n m : ℕ} {t t₀ t₁ : tree α β} (x : α) {z : zipper α β}
+variables {n m : ℕ} {pk : option α} {t t₀ t₁ : tree α β} (x : α) {z : zipper α β}
 
 section defns
 
@@ -136,20 +100,20 @@ inductive zipper_height (m : ℕ) : ℕ → zipper α β → Prop
 lemma with_height_close
   (h : with_height n t)
   (h' : zipper_height m n z) :
-  with_height m (close z t) ∨ with_height (succ m) (close z t) :=
+  with_height m (close z pk t) ∨ with_height (succ m) (close z pk t) :=
 begin
   left,
-  induction h' generalizing t; dsimp [close],
-  repeat { assumption <|> constructor <|> apply h'_ih },
+  induction h' generalizing t pk; dsimp [close] at *,
+  repeat { apply h'_ih <|> assumption <|> constructor },
 end
 
 lemma with_height_split
   (h₀ : with_height n t₀)
   (h₁ : with_height n t₁)
   (h' : zipper_height m n z) :
-  with_height m (split z t₀ x t₁) ∨ with_height (succ m) (split z t₀ x t₁) :=
+  with_height m (split z pk t₀ x t₁) ∨ with_height (succ m) (split z pk t₀ x t₁) :=
 begin
-  induction h' generalizing t₀ x t₁; dsimp [split],
+  induction h' generalizing t₀ x t₁ pk; dsimp [split],
   { right, constructor; assumption },
   repeat
   { apply with_height_close, constructor; assumption, assumption },
@@ -161,14 +125,14 @@ end defns
 
 section insert_height
 
-variables [decidable_linear_order α]
+variables [linear_order α]
 variables {k : α} {v : β}
 variables
   (h : zipper_height m n z)
   (h' : with_height n t)
 include h h'
 
-example : with_height m (insert k v z t) ∨ with_height (succ m) (insert k v z t) :=
+lemma with_height_insert : with_height m (insert k v z t) ∨ with_height (succ m) (insert k v z t) :=
 begin
   induction h' generalizing z,
   case two_three.with_height.leaf : k' v' z h
@@ -185,23 +149,14 @@ begin
     { assumption <|> apply h'_ih_a <|> apply h'_ih_a_1 <|> apply h'_ih_a_2 <|> constructor }, },
 end
 
-end insert_height
+lemma with_height_insert' (h' : with_height m t) : with_height m (insert' k v t) ∨ with_height (succ m) (insert' k v t) :=
+with_height_insert (by constructor) h'
 
--- def last : zipper α β → α
--- | nil := _
--- | (node2_0 a a_1 a_2) := last a
--- | (node2_1 a a_1 a_2) := two_three.last a
--- | (node3_0 a a_1 a_2 a_3 a_4) := last a
--- | (node3_1 a a_1 a_2 a_3 a_4) := two_three.last a
--- | (node3_2 a a_1 a_2 a_3 a_4) := two_three.last a
+end insert_height
 
 section defns
 
 variables [has_lt α] [has_le α]
-
-inductive above' : option α → α → Prop
-| nil {x} : above' none x
-| le {x y} : x < y → above' (some x) y
 
 inductive zipper_sorted : option α → zipper α β → option α → Prop
 | nil {a b} : zipper_sorted a zipper.nil b
@@ -212,10 +167,10 @@ inductive zipper_sorted : option α → zipper α β → option α → Prop
   above (last t₁) b →
   zipper_sorted a (node2_0 t₀ x t₁) (some x)
 | node2_1 {a b x t₀ t₁} :
+  zipper_sorted a t₁ b →
   below a (first t₀) →
   sorted' t₀ →
   last t₀ < x →
-  zipper_sorted a t₁ b →
   zipper_sorted (some x) (node2_1 t₀ x t₁) b
 
 | node3_0 {a b x y t₀ t₁ t₂} :
@@ -228,121 +183,164 @@ inductive zipper_sorted : option α → zipper α β → option α → Prop
   above (last t₂) b →
   zipper_sorted a (node3_0 t₀ x t₁ y t₂) (some x)
 | node3_1 {a b x y t₀ t₁ t₂} :
+  zipper_sorted a t₁ b →
   below a (first t₀) →
   sorted' t₀ →
   last t₀ < x →
-  zipper_sorted a t₁ b →
   y = first t₂ →
   sorted' t₂ →
   above (last t₂) b →
   zipper_sorted (some x) (node3_1 t₀ x t₁ y t₂) (some y)
 | node3_2 {a b x y t₀ t₁ t₂} :
+  zipper_sorted a t₂ b →
   below a (first t₀) →
   sorted' t₀ →
   last t₀ < x →
   x = first t₁ →
   sorted' t₁ →
   last t₁ < y →
-  zipper_sorted a t₂ b →
   zipper_sorted (some y) (node3_2 t₀ x t₁ y t₂) b
 
--- | node3 {x y t₀ t₁ t₂} :
---   last t₀ < x →
---   x = first t₁ →
---   last t₁ < y →
---   y = first t₂ →
---   sorted' t₀ →
---   sorted' t₁ →
---   sorted' t₂ →
---   sorted' (tree.node3 t₀ x t₁ y t₂)
+attribute [pp_nodot]
+  zipper_sorted.nil
+  zipper_sorted.node2_0
+  zipper_sorted.node2_1
+  zipper_sorted.node3_0
+  zipper_sorted.node3_1
+  zipper_sorted.node3_2
+  zipper.nil
+  zipper.node2_0
+  zipper.node2_1
+  zipper.node3_0
+  zipper.node3_1
+  zipper.node3_2
 
 end defns
 
 section insert_sorted
-variables  [decidable_linear_order α]
+-- variables {pk : option α}
+variables  [linear_order α]
 open two_three
 
 lemma sorted_close {a b}
+  (h' : zipper_sorted a z b)
   (h₀ : below a (first t))
+  (h₃ : below pk (first t))
   (h₁ : sorted' t)
   (h₂ : above (last t) b)
-  (h' : zipper_sorted a z b)
-  : sorted' (close z t) :=
+  : sorted' (close z pk t) :=
 begin
-  induction h' generalizing t,
+  induction h' generalizing t pk,
   all_goals
   { dsimp [close],
     saturate, subst_vars,
+    simp only * { fail_if_unchanged := ff },
     repeat
     { assumption <|> refl <|>
-      apply h'_ih <|> constructor }, },
+      apply h'_ih <|> constructor <|> cc }, },
 end
 
 lemma sorted_split {a x b}
+  (h' : zipper_sorted a z b)
   (h₀ : below a (first t₀))
+  (h₀ : below pk (first t₀))
   (h₁ : sorted' t₀)
   (h₂ : last t₀ < x)
   (h₃ : first t₁ = x)
   (h₃ : sorted' t₁)
   (h₄ : above (last t₁) b)
-  (h' : zipper_sorted a z b)
-  : sorted' (split z t₀ x t₁) :=
+  : sorted' (split z pk t₀ x t₁) :=
 begin
-  induction h' generalizing t₀ x t₁,
+  induction h' generalizing t₀ x t₁ pk,
   all_goals
   { dsimp [split],
     saturate, subst_vars,
+    simp only * { fail_if_unchanged := ff },
     repeat
     { assumption <|> refl <|>
       apply sorted_close <|>
       apply h'_ih <|> constructor }, },
 end
 
-lemma zipper_sorted_none : zipper_sorted none z none :=
-begin
-  induction z,
-  all_goals
-  { try { constructor,  } },
-end
-lemma zipper_sorted_none_of_zipper_sorted {a b} (h : zipper_sorted a z b) :
-  zipper_sorted a z none :=
-begin
-  induction h,
-  all_goals
-  { subst_vars, constructor }
-end
-lemma zipper_sorted_none_of_zipper_sorted' {a b} (h : zipper_sorted a z b) :
-  zipper_sorted none z b := sorry
+section tac
+open tactic
 
-variables {k : α} {v : β} {a b : option α}
+@[interactive]
+meta def simp_min : tactic unit :=
+run_bt $ do
+  x ← var,
+  y ← var,
+  (h, _) ← hyp_with ``(min %%x %%y),
+  bt_lift $ do
+  (pr, h) ← mcond (succeeds (is_def_eq x y))
+  (do p₀ ← to_expr ``(min %%x %%y = %%x),
+      n ← get_unused_name `h,
+      (h, _) ← local_proof n p₀ (applyc ``min_self),
+      pure (h, h))
+  (do p₀ ← to_expr ``(%%x ≤ %%y),
+      p₁ ← to_expr ``(%%y ≤ %%x),
+      n ← get_unused_name `h,
+      do { (h, _) ← local_proof n p₀ (assumption <|> applyc ``le_of_lt >> assumption),
+           pr ← mk_app ``min_eq_left [h],
+           pure (pr, h) } <|>
+        do { (h, _) ← local_proof n p₁ (assumption <|> applyc ``le_of_lt >> assumption),
+             pr ← mk_app ``min_eq_right [h],
+             pure (pr, h) }),
+   interactive.loc.apply
+     (λ h', try $ rewrite_hyp pr h' >> skip)
+     (try $ rewrite_target pr)
+     interactive.loc.wildcard,
+  skip
+
+end tac
+
+variables {k : α} {v : β} (a b : option α)
 variables (h : zipper_sorted a z b)
   (h' : sorted' t)
-  (h₀ : below a (first t))
+  (h₀ : below a (min k (first t)))
   (h₁ : above (last t) b)
-include h h' h₀ h₁
+  (h₂ : above k b)
+include h h' h₀ h₁ h₂
 
-example : sorted' (insert k v z t) :=
+lemma sorted_insert : sorted' (insert k v z t) :=
 begin
   induction h' generalizing z a b,
-  case two_three.sorted'.leaf : k' v' z h
-  { dsimp [insert], trichotomy k =? k',
-    repeat
-    { assumption <|> apply sorted_close <|> apply sorted_split <|>
-      apply zipper_sorted_none <|> constructor },
-
- },
-  case two_three.sorted'.node2 : h'_n h'_x h'_t₀ h'_t₁ _ h'_a h'_a_1 h'_ih_a h'_ih_a_1 z h a b
+  case two_three.sorted'.leaf : k' v' z a b h
+  { dsimp [insert], trichotomy k =? k' with h₂,
+    all_goals
+    { dsimp [first, last] at *,
+      subst_vars, simp_min, saturate,
+      apply sorted_split <|> apply sorted_close,
+      repeat
+      { assumption <|>
+        constructor <|>
+        simp_min <|> above } },  },
+  case two_three.sorted'.node2 : h'_x h'_t₀ h'_t₁ h'_a h'_a_1 h'_a_2 h'_a_3 h'_ih_a h'_ih_a_1 z a b h h₀ h₁ h₂
   { dsimp [insert], subst_vars, split_ifs,
-    repeat
-    { assumption <|> apply h'_ih_a <|> apply h'_ih_a_1 <|> constructor },
-    saturate,
-
- },
-  case two_three.sorted'.node3 : h'_n h'_x h'_y h'_t₀ h'_t₁ h'_t₂ h'_a h'_a_1 h'_a_2 h'_ih_a h'_ih_a_1 h'_ih_a_2 z h
-  { dsimp [insert], split_ifs,
-    repeat
-    { assumption <|> apply h'_ih_a <|> apply h'_ih_a_1 <|> apply h'_ih_a_2 <|> constructor }, },
+    all_goals
+    { dsimp [first] at *,
+      saturate, simp_min,
+      try { have : first h'_t₀ ≤ k, { chain_trans } },
+      apply h'_ih_a <|> apply h'_ih_a_1,
+      repeat
+      { assumption <|>
+        constructor <|>
+        simp_min <|> above, } } },
+  case two_three.sorted'.node3 : h'_x h'_y h'_t₀ h'_t₁ h'_t₂ h'_a h'_a_1 h'_a_2 h'_a_3 h'_a_4 h'_a_5 h'_a_6 h'_ih_a h'_ih_a_1 h'_ih_a_2 z a b h h₀ h₁ h₂
+  { dsimp [insert], subst_vars, split_ifs,
+    all_goals
+    { dsimp [first] at *,
+      saturate, simp_min,
+      try { have : first h'_t₀ ≤ k, { chain_trans } },
+      apply h'_ih_a <|> apply h'_ih_a_1 <|> apply h'_ih_a_2,
+      repeat
+      { assumption <|>
+        constructor <|>
+        simp_min <|> above, } } },
 end
+
+lemma sorted_insert' : sorted' (insert' k v t) :=
+by apply sorted_insert none none _ h'; constructor
 
 end insert_sorted
 
