src/backtrack.lean
@@ -1,0 +1,45 @@
+
+import control.monad.cont
+
+open tactic
+
+namespace tactic
+
+-- this should probably be PR-ed
+meta def bt_tac (α : Type) :=
+∀ r, cont_t r tactic α
+
+meta instance : monad bt_tac :=
+{ pure := λ α x r, pure x,
+  bind := λ α β x f r, x r >>= λ a, f a r }
+
+meta instance bt_tac.alternative : alternative bt_tac :=
+{ failure := λ α r _, failure,
+  orelse  := λ α x y r f, x _ f <|> y _ f }
+
+meta def run_bt {α} (x : bt_tac α) : tactic α :=
+x _ pure
+
+meta def bt_lift {α} (x : tactic α) : bt_tac α :=
+λ r f, x >>= f
+
+meta def var : bt_tac expr :=
+bt_lift mk_mvar
+
+meta def hyp (p : pexpr) : bt_tac expr := do
+p ← bt_lift $ to_expr p,
+ls ← bt_lift local_context,
+ls.mfirst $ λ h, bt_lift $ do
+  t ← infer_type h,
+  h <$ unify t p
+
+meta def hyp_with (p : pexpr) : bt_tac (expr × expr) := do
+p ← bt_lift $ to_expr p,
+ls ← bt_lift local_context,
+ls.mfirst $ λ h, bt_lift $ do
+  t ← infer_type h,
+  e ← kabstract t p,
+  guard $ e.has_var,
+  pure (h, e)
+
+end tactic
