src/basic.lean
@@ -1,0 +1,114 @@
+
+import tactic.default .tactic
+universes u v w
+
+namespace two_three
+
+variables (α : Type u) (β : Type v) {γ : Type w}
+
+inductive tree
+| leaf (k : α) (v : β)
+| node2 (t₀ : tree) (x : α) (t₁ : tree)
+| node3 (t₀ : tree) (x : α) (t₁ : tree) (y : α) (t₂ : tree)
+
+open tree nat
+
+variables {α β}
+
+def first : tree α β → α
+| (tree.leaf x _) := x
+| (tree.node2 t₀ x _) := first t₀
+| (tree.node3 t₀ x _ _ _) := first t₀
+
+def last : tree α β → α
+| (tree.leaf x _) := x
+| (tree.node2 _ x t₁) := last t₁
+| (tree.node3 t₀ x _ _ t₂) := last t₂
+
+section defs
+variables [has_le α] [has_lt α]
+
+open tree nat
+
+inductive below : option α → α → Prop
+| nil {x} : below none x
+| eq {x} : below (some x) x
+
+inductive above : α → option α → Prop
+| nil {x} : above x none
+| le {x y} : x < y → above x (some y)
+
+inductive sorted' : tree α β → Prop
+| leaf {k v} : sorted' (tree.leaf k v)
+| node2 {x t₀ t₁} :
+  last t₀ < x →
+  x = first t₁ →
+  sorted' t₀ →
+  sorted' t₁ →
+  sorted' (tree.node2 t₀ x t₁)
+| node3 {x y t₀ t₁ t₂} :
+  last t₀ < x →
+  x = first t₁ →
+  last t₁ < y →
+  y = first t₂ →
+  sorted' t₀ →
+  sorted' t₁ →
+  sorted' t₂ →
+  sorted' (tree.node3 t₀ x t₁ y t₂)
+
+inductive with_height : ℕ → tree α β → Prop
+| leaf {k v} : with_height 0 (tree.leaf k v)
+| node2 {n x t₀ t₁} :
+  with_height n t₀ →
+  with_height n t₁ →
+  with_height (succ n) (tree.node2 t₀ x t₁)
+| node3 {n x y t₀ t₁ t₂} :
+  with_height n t₀ →
+  with_height n t₁ →
+  with_height n t₂ →
+  with_height (succ n) (tree.node3 t₀ x t₁ y t₂)
+
+end defs
+
+local attribute [simp] first last
+
+variables [linear_order α]
+
+lemma first_le_last_of_sorted {t : tree α β} (h : sorted' t) :
+  first t ≤ last t :=
+begin
+  induction h; subst_vars; dsimp [first, last],
+  { refl },
+  repeat { solve_by_elim [le_of_lt] <|> transitivity },
+end
+
+lemma eq_of_below {x : option α} {y : α} (h : below x y) : x.get_or_else y = y :=
+by cases h; refl
+
+lemma above_of_above_of_le {x y : α} {k}
+  (h : x ≤ y) (h' : above y k) : above x k :=
+by cases h'; constructor; solve_by_elim [lt_of_le_of_lt]
+
+@[interactive]
+meta def interactive.saturate : tactic unit := do
+tactic.interactive.casesm (some ()) [``(above _ (some _)), ``(below (some _) _)],
+tactic.find_all_hyps ``(sorted' _) $ λ h, do
+{ n ← tactic.get_unused_name `h,
+  tactic.mk_app ``first_le_last_of_sorted [h] >>= tactic.note n none,
+  tactic.skip },
+tactic.find_all_hyps ``(below _ _) $ λ h, do
+{ n ← tactic.get_unused_name `h,
+  tactic.mk_app ``eq_of_below [h] >>= tactic.note n none,
+  tactic.skip },
+tactic.find_all_hyps ``(¬ _ < _) $ λ h, do
+{ tactic.mk_app ``le_of_not_gt [h] >>= tactic.note h.local_pp_name none,
+  tactic.clear h,
+  tactic.skip }
+
+@[interactive]
+meta def interactive.above : tactic unit := do
+tactic.find_hyp ``(above _ _) $ λ h, do
+  tactic.refine ``(above_of_above_of_le _ %%h),
+  tactic.interactive.chain_trans
+
+end two_three
